DesugarScopedVars.dfy
@@ -11,21 +11,21 @@ module DesugarScopedVars {
   import Util
   import opened Wrappers
 
-  predicate RelState<V>(m: map<var_name, var_name>, s1: map<var_name, V>, s2: map<var_name, V>)
+  predicate {:opaque} RelState<V>(m: map<var_name, var_name>, s1: map<var_name, V>, s2: map<var_name, V>)
   {
     (forall k | k in m.Keys :: Maps.Get(s1, k) == Maps.Get(s2, m[k]))
   }
 
-  lemma RelStateEmpty<V>(s1: map<var_name, V> , s2: map<var_name, V>)
+ lemma {:verify false} RelStateEmpty<V>(s1: map<var_name, V> , s2: map<var_name, V>)
   ensures RelState(map[], s1, s2)
-  { }
+ { reveal RelState(); }
 
-  predicate RelPred<A(!new)>(m: map<var_name, var_name>, post1: Predicate<A>, post2: Predicate<A>)
+  predicate {:opaque} RelPred<A(!new)>(m: map<var_name, var_name>, post1: Predicate<A>, post2: Predicate<A>)
   {
     forall s, s' | RelState(m, s, s') :: post1(s) == post2(s')
   }
 
-  predicate RelPost<A(!new)>(m: map<var_name, var_name>, post1: WpPostShallow<A>, post2: WpPostShallow<A>)
+  predicate {:opaque} RelPost<A(!new)>(m: map<var_name, var_name>, post1: WpPostShallow<A>, post2: WpPostShallow<A>)
   {
     && post1.scopes.Keys == post2.scopes.Keys
     && RelPred(m, post1.normal, post2.normal)
@@ -35,17 +35,18 @@ module DesugarScopedVars {
 
   function method MultiSubstExpr(e: Expr, varMapping: map<var_name, var_name>): Expr
 
-  lemma MultiSubstExprSpec<A(!new)>(a: absval_interp<A>, varMapping: map<var_name, var_name>, e: Expr, s1: state<A>, s2: state<A>)
+ lemma {:verify false} MultiSubstExprSpec<A(!new)>(a: absval_interp<A>, varMapping: map<var_name, var_name>, e: Expr, s1: state<A>, s2: state<A>)
     requires forall x | x in e.FreeVars() :: 
       && (x in varMapping.Keys ==> Maps.Get(s1, x) == Maps.Get(s2, varMapping[x]))
       && (x !in varMapping.Keys ==> Maps.Get(s1, x) == Maps.Get(s2, x))
     ensures EvalExpr(a, e, s1) == EvalExpr(a, MultiSubstExpr(e, varMapping), s2)
   
-  lemma MultiSubstExprSpec2<A(!new)>(a: absval_interp<A>, varMapping: map<var_name, var_name>, e: Expr, s1: state<A>, s2: state<A>)
+ lemma {:verify false} MultiSubstExprSpec2<A(!new)>(a: absval_interp<A>, varMapping: map<var_name, var_name>, e: Expr, s1: state<A>, s2: state<A>)
     requires RelState(varMapping, s1, s2)
     requires e.FreeVars() <= varMapping.Keys
     ensures EvalExpr(a, e, s1) == EvalExpr(a, MultiSubstExpr(e, varMapping), s2)
   {
+    reveal RelState();
     MultiSubstExprSpec(a, varMapping, e, s1, s2);
   }
 
@@ -60,16 +61,15 @@ module DesugarScopedVars {
       var newRHS := MultiSubstExpr(e, varMapping);
       Assign(newLHS, t, newRHS)
     case Havoc(varDecls) =>
-      var varDecls' := Sequences.Map( 
-        (vDecl : (var_name, Ty)) => 
-          if vDecl.0 in varMapping.Keys then (varMapping[vDecl.0], vDecl.1) else vDecl,
-        varDecls);
+      var f := (vDecl : (var_name, Ty)) => 
+          if vDecl.0 in varMapping.Keys then (varMapping[vDecl.0], vDecl.1) else vDecl;
+      var varDecls' := Sequences.Map(f, varDecls);
       Havoc(varDecls')
     case SeqSimple(c1, c2)  =>
       SeqSimple(SubstSimpleCmd(c1, varMapping), SubstSimpleCmd(c2, varMapping))
   }
 
-  lemma ForallVarDeclsRel<A(!new)>(
+ lemma {:verify false} {:induction false} ForallVarDeclsRel<A(!new)>(
     a: absval_interp<A>, 
     varDecls: seq<(var_name, Ty)>, 
     varMapping: map<var_name, var_name>, 
@@ -77,20 +77,91 @@ module DesugarScopedVars {
     p2: Predicate<A>)
     requires RelPred(varMapping, p1, p2)
     requires GetVarNames(varDecls) <= varMapping.Keys
+    requires Maps.Injective(varMapping)
     ensures 
-      var varDecls' := Sequences.Map((vDecl : (var_name, Ty)) => (varMapping[vDecl.0], vDecl.1), varDecls);
-      RelPred(varMapping, ForallVarDeclsShallow(a, varDecls, p1), ForallVarDeclsShallow(a, varDecls, p2))
+      var f := (vDecl : (var_name, Ty)) => 
+          if vDecl.0 in varMapping.Keys then (varMapping[vDecl.0], vDecl.1) else vDecl;
+      var varDecls' := Sequences.Map(f, varDecls);
+      RelPred(varMapping, ForallVarDeclsShallow(a, varDecls, p1), ForallVarDeclsShallow(a, varDecls', p2))
   {
-    forall s1, s2 | RelState(varMapping, s1, s2)
-    ensures ForallVarDeclsShallow(a, varDecls, p1)(s1) == ForallVarDeclsShallow(a, varDecls, p2)(s2)
-    {
-      if |varDecls| > 0 {
+    var f := (vDecl : (var_name, Ty)) => 
+        if vDecl.0 in varMapping.Keys then (varMapping[vDecl.0], vDecl.1) else vDecl;
+    var varDecls' := Sequences.Map(f, varDecls);
+    if |varDecls| == 0 {
+      //trivial
+      reveal ForallVarDeclsShallow();
+      assert ForallVarDeclsShallow(a, varDecls, p1) == p1;
+    } else {
+      var (x,t) := varDecls[0];
+      var x' := varMapping[x];
 
+      var f := (vDecl : (var_name, Ty)) => 
+          if vDecl.0 in varMapping.Keys then (varMapping[vDecl.0], vDecl.1) else vDecl;
+      var varDecls' := Sequences.Map(f, varDecls);
+
+      forall s1: map<var_name, Val<A>>, s2, v: Val<A> | RelState(varMapping, s1, s2) && TypeOfVal(a, v) == t
+        ensures ForallVarDeclsShallow(a, varDecls[1..], p1)(s1[x := v]) == ForallVarDeclsShallow(a, varDecls'[1..], p2)(s2[x' := v])
+      {
+        assert RelState(varMapping, s1[x := v], s2[x' := v]) by {
+          RelStatePreserve(varMapping, s1, s2, x, v);
+        }
+        ForallVarDeclsRel(a, varDecls[1..], varMapping, p1, p2);
+        reveal RelPred();
+
+        assert varDecls'[1..] == Sequences.Map(f, varDecls[1..]);
       }
+
+      reveal ForallVarDeclsShallow();
     }
   }
 
-  lemma SubstSimpleCmdCorrect<A(!new)>(a: absval_interp<A>, sc: SimpleCmd, varMapping: map<var_name, var_name>, 
+ lemma {:verify false} ForallVarDeclsRel2<A(!new)>(
+    a: absval_interp<A>, 
+    varDecls: seq<(var_name, Ty)>, 
+    varMapping: map<var_name, var_name>, 
+    p1: Predicate<A>,
+    p2: Predicate<A>,
+    s1: state<A>,
+    s2: state<A>)
+    requires RelPred(varMapping, p1, p2)
+    requires RelState(varMapping, s1, s2)
+    requires GetVarNames(varDecls) <= varMapping.Keys
+    requires Maps.Injective(varMapping)
+    ensures 
+      var f := (vDecl : (var_name, Ty)) => 
+          if vDecl.0 in varMapping.Keys then (varMapping[vDecl.0], vDecl.1) else vDecl;
+      var varDecls' := Sequences.Map(f, varDecls);
+      ForallVarDeclsShallow(a, varDecls, p1)(s1) ==  ForallVarDeclsShallow(a, varDecls', p2)(s2)
+  {
+    ForallVarDeclsRel(a, varDecls, varMapping, p1, p2);
+    reveal RelPred();
+  }
+
+ lemma {:verify false} RelStatePreserve<V>(varMapping: map<var_name, var_name>, s1: map<var_name, V>, s2: map<var_name, V>, x: var_name, v: V)
+ requires RelState(varMapping, s1, s2)
+ requires Maps.Injective(varMapping)
+ requires x in varMapping.Keys
+ ensures RelState(varMapping, s1[x := v], s2[varMapping[x] := v])
+ {
+  reveal RelState();
+  var x' := varMapping[x];
+  forall k | k in varMapping.Keys 
+  ensures Maps.Get(s1[x := v], k) == Maps.Get(s2[varMapping[x] := v], varMapping[k])
+  {
+    var k' := varMapping[k];
+    if k != x {
+      calc {
+        Maps.Get(s1[x := v], k);
+        Maps.Get(s1, k);
+        Maps.Get(s2, k');
+        { reveal Maps.Injective(); }
+        Maps.Get(s2[x' := v], k');
+      }
+    }
+  }
+ }
+
+ lemma {:verify false} {:induction false} SubstSimpleCmdCorrect<A(!new)>(a: absval_interp<A>, sc: SimpleCmd, varMapping: map<var_name, var_name>, 
     post1: Predicate<A>, post2: Predicate<A>)
     requires RelPred(varMapping, post1, post2)
     requires sc.WellFormedVars(varMapping.Keys)
@@ -105,55 +176,85 @@ module DesugarScopedVars {
     forall s1:map<var_name, Val<A>>, s2 | RelState(varMapping, s1, s2)
       ensures pre1(s1) == pre2(s2)
     {
-      match sc
-      case Assume(e) => 
-        MultiSubstExprSpec2(a, varMapping, e, s1, s2);
-      case Assert(e) => 
-        MultiSubstExprSpec2(a, varMapping, e, s1, s2);
-      case Assign(x, t, e) =>
-        var e' := MultiSubstExpr(e, varMapping);
-        var v1Opt := EvalExpr(a, e, s1);
-        var v2Opt := EvalExpr(a, e', s2);
-        assert v1Opt == v2Opt by {
+      reveal RelPred();
+      match sc {
+        case Skip => 
+        case Assume(e) => 
           MultiSubstExprSpec2(a, varMapping, e, s1, s2);
-        }
+        case Assert(e) => 
+          reveal RelPred();
+          MultiSubstExprSpec2(a, varMapping, e, s1, s2);
+        case Assign(x, t, e) =>
+          var e' := MultiSubstExpr(e, varMapping);
+          var v1Opt := EvalExpr(a, e, s1);
+          var v2Opt := EvalExpr(a, e', s2);
+          assert v1Opt == v2Opt by {
+            MultiSubstExprSpec2(a, varMapping, e, s1, s2);
+          }
 
-        if(v1Opt.Some?) {
-          var v := v1Opt.value;
-          var x' := varMapping[x];
+          if(v1Opt.Some?) {
+            var v := v1Opt.value;
+            var x' := varMapping[x];
 
-          assert RelState(varMapping, s1[x := v], s2[x' := v]) by {
-            forall k | k in varMapping.Keys 
-            ensures Maps.Get(s1[x := v], k) == Maps.Get(s2[x' := v], varMapping[k])
-            {
-              var k' := varMapping[k];
-              if k != x {
-                calc {
-                  Maps.Get(s1[x := v], k);
-                  Maps.Get(s1, k);
-                  Maps.Get(s2, k');
-                  { reveal Maps.Injective(); }
-                  Maps.Get(s2[x' := v], k');
-                }
-              }
+            assert RelState(varMapping, s1[x := v], s2[x' := v]) by {
+              RelStatePreserve(varMapping, s1, s2, x, v);
             }
           }
-        }
-      case Havoc(vDecls)  => 
+        case Havoc(vDecls) => 
+          var f := 
+            (vDecl : (var_name, Ty)) => 
+                  if vDecl.0 in varMapping.Keys then (varMapping[vDecl.0], vDecl.1) else vDecl;
+          var vDecls' := Sequences.Map(f, vDecls);
+          
+          calc {
+            WpShallowSimpleCmd(a, Havoc(vDecls), post1)(s1);
+            ForallVarDeclsShallow(a, vDecls, post1)(s1);
+            { ForallVarDeclsRel2(a, vDecls, varMapping, post1, post2, s1, s2); }
+            ForallVarDeclsShallow(a, vDecls', post2)(s2);
+            WpShallowSimpleCmd(a, Havoc(vDecls'), post2)(s2);
+            WpShallowSimpleCmd(a, SubstSimpleCmd(Havoc(vDecls), varMapping), post2)(s2);
+          }
+        case SeqSimple(sc1, sc2) =>
+          var sc1' := SubstSimpleCmd(sc1, varMapping);
+          var sc2' := SubstSimpleCmd(sc2, varMapping);
 
-      case _ => assume false;
+          var post1' := WpShallowSimpleCmd(a, sc2, post1);
+          var post2' := WpShallowSimpleCmd(a, sc2', post2);
+
+
+          calc {
+            WpShallowSimpleCmd(a, SeqSimple(sc1, sc2), post1)(s1);
+            WpShallowSimpleCmd(a, sc1, post1')(s1);
+            { 
+              assert RelPred(varMapping, post1', post2') by{
+                SubstSimpleCmdCorrect(a, sc2, varMapping, post1, post2);
+              }
+              SubstSimpleCmdCorrect(a, sc1, varMapping, post1', post2'); 
+            }
+            WpShallowSimpleCmd(a, sc1', post2')(s2);
+            WpShallowSimpleCmd(a, SeqSimple(sc1', sc2'), post2)(s2);
+          }
+      }
     }
   }
 
 
   function method CreateUniqueName(names: set<var_name>): var_name
     ensures CreateUniqueName(names) !in names
+  
+  const SEP : string := "#";
 
-  function method CreateUniqueVarDecls(varDecls: seq<(var_name, Ty)>, usedNames: set<var_name>) : seq<(var_name,Ty)>
+  function method VersionedName(name: string, n: nat) : string
+  {
+    name + Util.NatToString(n) + SEP
+  }
+
+  function method CreateUniqueVarDecls(varDecls: seq<(var_name, Ty)>, usedNames: set<var_name>, counter: nat) : seq<(var_name,Ty)>
     ensures 
-      var res := CreateUniqueVarDecls(varDecls, usedNames);
+      var res := CreateUniqueVarDecls(varDecls, usedNames, counter);
       |varDecls| == |res|
   {
+    /*
     var f := (varDecl:(var_name, Ty), res: seq<(var_name, Ty)>) => (
       var (x, t) := varDecl;
 
@@ -168,8 +269,18 @@ module DesugarScopedVars {
     Sequences.LemmaInvFoldRight(inv, step, f, [], varDecls);
 
     var res := Sequences.FoldRight(f, varDecls, []);
+    */
 
-    res
+    /** TODO
+      Currently, a suffix is added to every variable even if there are no clashes. 
+      This makes it harder to read the target output. It would be nice if one could 
+      reuse a name if it does not clash with anything else that has been so far. 
+      Doing this would require a fold to avoid updating the counter if a name is 
+      reused.
+     */
+
+    // DISCUSS
+    seq(|varDecls|, i => (VersionedName(varDecls[i].0, counter+i), varDecls[i].1))
   }
 
   function method ConvertVDeclsToSubstMap(varDecls: seq<(var_name, Ty)>, varDecls': seq<(var_name, Ty)>) : map<var_name, var_name>
@@ -190,8 +301,12 @@ module DesugarScopedVars {
   function method DesugarScopedVars(
     c: Cmd, 
     substMap: map<var_name, var_name>, 
-    usedVars: set<var_name>,
-    ghost seqSubstMap: seq<(var_name, Ty)>): (Cmd, set<var_name>)
+    usedVars: (set<var_name>,nat),
+    ghost seqSubstMap: seq<(var_name, Ty)>): (Cmd, (set<var_name>, nat))
+    /*requires substMap.Values <= set c,x | x in substMap.Keys && 0 < c < usedVars.1 :: VersionedName(x, c)
+    requires forall x | x in substMap.Keys :: exists c : nat :: c <= usedVars.1 && substMap[x] == VersionedName(x, c)
+    ensures 
+      forall x | x in substMap.Keys :: exists c : nat :: c <= usedVars.1 && substMap[x] == VersionedName(x, c)*/
   {
     match c
     case SimpleCmd(sc) => (SimpleCmd(SubstSimpleCmd(sc, substMap)), usedVars)
@@ -201,8 +316,8 @@ module DesugarScopedVars {
       var (c2', usedVars2') := DesugarScopedVars(c2, substMap, usedVars1', seqSubstMap);
       (Seq(c1', c2'), usedVars2')
     case Scope(optLabel, varDecls, body) =>
-      var varDecls' := CreateUniqueVarDecls(varDecls, usedVars);
-      var usedVars' := usedVars + GetVarNames(varDecls');
+      var varDecls' := CreateUniqueVarDecls(varDecls, usedVars.0, usedVars.1);
+      var usedVars' := (usedVars.0 + GetVarNames(varDecls'), usedVars.1 + |varDecls'|);
       var substMap' := substMap + ConvertVDeclsToSubstMap(varDecls, varDecls');
       var (body'', usedVars'') := DesugarScopedVars(body, substMap, usedVars', seqSubstMap);
       (Scope(optLabel, varDecls', body''), usedVars'')
@@ -213,6 +328,73 @@ module DesugarScopedVars {
       (If(None, thn', els'), usedVars'')
     case _ => (c, usedVars) //TODO (precondition should eliminate this case)
   }
+
+  function method RemoveScopedVars(c: Cmd): (Cmd, (seq<(var_name, Ty)>))
+    /*requires substMap.Values <= set c,x | x in substMap.Keys && 0 < c < usedVars.1 :: VersionedName(x, c)
+    requires forall x | x in substMap.Keys :: exists c : nat :: c <= usedVars.1 && substMap[x] == VersionedName(x, c)
+    ensures 
+      forall x | x in substMap.Keys :: exists c : nat :: c <= usedVars.1 && substMap[x] == VersionedName(x, c)*/
+  {
+    match c
+    case SimpleCmd(sc) => (c, [])
+    case Break(_) => (c, [])
+    case Seq(c1, c2) => 
+      var (c1', decls1) := RemoveScopedVars(c1);
+      var (c2', decls2) := RemoveScopedVars(c2);
+      (Seq(c1', c2'), decls1 + decls2)
+    case Scope(optLabel, varDecls, body) =>
+      var (body', declsBody) := RemoveScopedVars(body);
+      (Scope(optLabel, [], body'), varDecls + declsBody)
+    case If(None, thn, els) => 
+      //TODO: make sure If(Some(...)) has been desugared
+      var (thn', declsThn) := RemoveScopedVars(thn);
+      var (els', declsEls) := RemoveScopedVars(els);
+      (If(None, thn', els'), declsThn + declsEls)
+    case _ => (c, []) //TODO (precondition should eliminate this case)
+  }
+
+  lemma RemoveScopedVarsCorrect<A(!new)>(a: absval_interp<A>, c: Cmd, post: WpPostShallow<A>)
+    requires 
+      var (c', decls) := RemoveScopedVars(c);
+      LabelsWellDefAux(c, post.scopes.Keys) && LabelsWellDefAux(c', post.scopes.Keys)
+    ensures 
+      var (c', decls) := RemoveScopedVars(c);
+      forall s :: WpShallow(a, c, post)(s) == ForallVarDeclsShallow(a, decls, WpShallow(a, c', ResetVarsPost(a, decls, post, s)))(s)
+  
+  /*
+  lemma ScopeNoneSemantics<A(!new)>(a: absval_interp<A>, varDecls: seq<(var_name, Ty)>, body: Cmd, post: WpPostShallow<A>)
+      requires LabelsWellDefAux(body, post.scopes.Keys)
+    ensures
+      forall s : state<A> :: 
+        WpShallow(a, Scope(None, varDecls, body), post)(s) ==
+        ForallVarDeclsShallow(a, varDecls, WpShallow(a, body, ResetVarsPost(a, varDecls, WpPostShallow(post.normal, post.normal, post.scopes), s)))(s)
+    { 
+      assume false;
+    }
+  */
+
+  lemma ScopeSemantics<A(!new)>(a: absval_interp<A>, optLabel: Option<lbl_name>, varDecls: seq<(var_name, Ty)>, body: Cmd, post: WpPostShallow<A>, s: state<A>)
+    requires LabelsWellDefAux(Scope(optLabel, varDecls, body), post.scopes.Keys)
+    ensures
+        WpShallow(a, Scope(optLabel, varDecls, body), post)(s) ==
+        ForallVarDeclsShallow(a, varDecls, WpShallow(a, Scope(optLabel, [], body), ResetVarsPost(a, varDecls, post, s)))(s)
+  {
+      var updatedScopes := 
+        if optLabel.Some? then 
+          post.scopes[optLabel.value := post.normal]
+        else post.scopes;
+
+    assert updatedScopes.Keys == if optLabel.Some? then {optLabel.value} + post.scopes.Keys else post.scopes.Keys;
+    var post' := WpPostShallow(post.normal, post.normal, updatedScopes);
+    calc {
+      WpShallow(a, Scope(optLabel, varDecls, body), post)(s);
+      ForallVarDeclsShallow(a, varDecls, WpShallow(a, body, ResetVarsPost(a, varDecls, post', s)))(s);
+      { assert ResetVarsPost(a, [], ResetVarsPost(a, varDecls, post', s), s) == ResetVarsPost(a, varDecls, post', s); }
+      ForallVarDeclsShallow(a, varDecls, WpShallow(a, body, ResetVarsPost(a, [], ResetVarsPost(a, varDecls, post', s), s)))(s);
+      ForallVarDeclsShallow(a, varDecls, WpShallow(a, Scope(optLabel, [], body), ResetVarsPost(a, varDecls, post, s)))(s);
+    }
+  }
+   
 
   function RenameVarsState<V>(m: map<var_name, var_name>, s: map<var_name, V>) : map<var_name, V>
     ensures 
@@ -241,16 +423,17 @@ module DesugarScopedVars {
     WpPostShallow(RenameVarsPred(m, post.normal), RenameVarsPred(m, post.currentScope), newScopes)
   }
 
-  lemma DesugarScopedVarsCorrect<A(!new)>(
+ lemma {:verify true} DesugarScopedVarsCorrect<A(!new)>(
     a: absval_interp<A>,
     c: Cmd, 
     substMap: map<var_name, var_name>, 
-    usedVars: set<var_name>,
+    usedVars: (set<var_name>, nat),
     seqSubstMap: seq<(var_name, Ty)>,
     post1: WpPostShallow<A>,
-    post2: WpPostShallow<A>,
-    s: state<A>)
+    post2: WpPostShallow<A>)
+  requires c.WellFormedVars(substMap.Keys)
   requires |seqSubstMap| == |substMap.Keys|
+  requires Maps.Injective(substMap)
   requires 
     var (c', usedVars') := DesugarScopedVars(c, substMap, usedVars, seqSubstMap);
     && LabelsWellDefAux(c, post1.scopes.Keys) 
@@ -261,5 +444,36 @@ module DesugarScopedVars {
   ensures 
     var (c', usedVars') := DesugarScopedVars(c, substMap, usedVars, seqSubstMap);
     RelPred(substMap, WpShallow(a, c, post1), WpShallow(a, c', post2))
+  /** proof sketch notes:  
+    for scopes case, will have to show that the updated substMap remains injective 
+  */
+ {
+   reveal RelPost();
+   match c {
+    case SimpleCmd(sc) =>
+      SubstSimpleCmdCorrect(a, sc, substMap, post1.normal, post2.normal);
+    case Break(_) =>
+    case Seq(c1, c2) => 
+      var (c1', usedVars1') := DesugarScopedVars(c1, substMap, usedVars, seqSubstMap);
+      var (c2', usedVars2') := DesugarScopedVars(c2, substMap, usedVars1', seqSubstMap);
+
+      var post1' := WpPostShallow(WpShallow(a, c2, post1), post1.currentScope, post1.scopes);
+      var post2' := WpPostShallow(WpShallow(a, c2', post2), post2.currentScope, post2.scopes);
+
+      assert RelPost(substMap, post1', post2') by {
+        assert RelPred(substMap, WpShallow(a, c2, post1), WpShallow(a, c2', post2)) by {
+          DesugarScopedVarsCorrect(a, c2, substMap, usedVars1', seqSubstMap, post1, post2);
+        }
+      }
+
+      assert RelPred(substMap, WpShallow(a, c1, post1'), WpShallow(a, c1', post2')) by {
+        DesugarScopedVarsCorrect(a, c1, substMap, usedVars, seqSubstMap, post1', post2');
+      }
+    case Scope(labelName, varDecls, body) => assume false;
+    case If(guard, thn, els) => assume false;
+    case Loop(invariants, body) => assume false;
+   }
+ }
+
 
 }
